Add natural number type

syntax.sig
@@ -6,10 +6,10 @@ tApp : tm -> tm -> tm
 tPi : tm -> (tm -> tm) -> tm
 tVoid : tm
 tUniv : nat -> tm
-tTrue : tm
-tFalse : tm
-tIf : tm -> tm -> tm -> tm
-tBool : tm
 tEq : tm -> tm -> tm -> tm
 tJ : tm -> tm -> tm -> tm -> tm
 tRefl : tm
+tZero : tm
+tSuc : tm -> tm
+tInd : tm -> (tm -> tm -> tm) -> tm -> tm
+tNat : tm
